Veil/Core/Tools/ModelChecker/ConcreteNew/SequentialLemmas.lean
@@ -2,14 +2,14 @@ import Veil.Core.Tools.ModelChecker.ConcreteNew.SearchContext
 
 namespace Veil.ModelChecker.Concrete
 
-variable {ρ σ κ σₕ : Type}
+variable {ρ σ κ σₕ asm : Type}
   [fp : StateFingerprint σ σₕ]
-  [BEq κ] [Hashable κ]
+  [ActionStatUpdate κ asm]
   {th : ρ}
   (sys : EnumerableTransitionSystem ρ (List ρ) σ (List σ) Int κ (List (κ × ExecutionOutcome Int σ)) th)
   (params : SearchParameters ρ σ)
 
-def SequentialSearchContext.initial : SequentialSearchContext σ κ σₕ :=
+def SequentialSearchContext.initial : SequentialSearchContext σ κ σₕ asm :=
   let iss := sys.initStates
   (BaseSearchContext.initial iss, fQueue.ofList (iss.map (fun s => ⟨fp.view s, s, 0⟩)))
 
@@ -22,7 +22,7 @@ theorem SequentialSearchContextInvariants.initial :
 in transit to having no state in transit, provided that all successfully
 reachable neighbors of `curr` in transit have been seen. -/
 theorem SequentialSearchContextInvariants.finish_stateInTransit
-  {sctx : SequentialSearchContext σ κ σₕ}
+  {sctx : SequentialSearchContext σ κ σₕ asm}
   {curr : σ}
   (sctx_invs : SequentialSearchContextInvariants sys params (.some curr) sctx)
   (h_neighbors_seen : ∀ l v, (l, ExecutionOutcome.success v) ∈ sys.tr th curr →
@@ -37,7 +37,7 @@ theorem SequentialSearchContextInvariants.finish_stateInTransit
   subst u ; eapply h_neighbors_seen ; assumption
 
 theorem SequentialSearchContext.bfs_completeness
-  {sctx : SequentialSearchContext σ κ σₕ}
+  {sctx : SequentialSearchContext σ κ σₕ asm}
   (sctx_invs : SequentialSearchContextInvariants sys params .none sctx)
   (h_explore_all : sctx.1.finished = some (.exploredAllReachableStates))
   (h_view_inj : Function.Injective fp.view) :
